Auto/Lib/HEqExtra.lean
@@ -3,11 +3,11 @@ namespace Auto
 theorem heq_of_cast_eq : ∀ (e : α = β) (_ : cast e a = a'), HEq a a'
   | rfl, h => Eq.recOn h (HEq.refl _)
 
-def HEq.tyEq {α β : Sort u} (x : α) (y : β) (H : HEq x y) : α = β :=
+theorem HEq.tyEq {α β : Sort u} (x : α) (y : β) (H : HEq x y) : α = β :=
   match β, y, H with
   | .(α), .(x), HEq.refl _ => Eq.refl _
 
-def HEq.funext {γ : Sort u} {α β : γ → Sort v}
+theorem HEq.funext {γ : Sort u} {α β : γ → Sort v}
   (x : ∀ (u : γ), α u) (y : ∀ (u : γ), β u) (H : ∀ u, HEq (x u) (y u)) : HEq x y :=
   (fun αβEq : α = β =>
     match β, αβEq with
